small tweaks to LR, progress in proving the allocation of interp instance

theories/iris_robust_examples.v
@@ -3,9 +3,8 @@ From iris.program_logic Require Import language.
 From iris.proofmode Require Import base tactics classes.
 From iris.base_logic Require Export gen_heap ghost_map proph_map.
 From iris.base_logic.lib Require Export fancy_updates.
-From iris.bi Require Export weakestpre.
 Require Export iris iris_locations iris_properties iris_atomicity stdpp_aux.
-Require Export iris_rules iris_fundamental.
+Require Export iris_host iris_rules iris_fundamental iris_wp.
 Require Export datatypes host operations properties opsem.
 
 Set Implicit Arguments.
@@ -15,7 +14,7 @@ Unset Printing Implicit Defensive.
 Close Scope byte_scope.
 
 Notation "{{{ P }}} es {{{ v , Q }}}" :=
-  (∀ Φ, P -∗ (∀ v, Q -∗ Φ v) -∗ WP es @ NotStuck ; ⊤ {{ v, Φ v }}) (at level 50).
+  (∀ Φ, P -∗ (∀ v, Q -∗ Φ v) -∗ WP (es : iris.expr) @ NotStuck ; ⊤ {{ v, Φ v }}) (at level 50).
 
 Ltac take_drop_app_rewrite n :=
   match goal with
@@ -43,7 +42,10 @@ Import DummyHosts.
 (* Example Programs *)
 Section Examples.
 
-  Context `{!wfuncG Σ, !wtabG Σ, !wtabsizeG Σ, !wmemG Σ, !wmemsizeG Σ, !wglobG Σ, !wframeG Σ, !logrel_na_invs Σ, HWP:host_program_logic}.
+  Import DummyHost.
+
+  Context `{!wfuncG Σ, !wtabG Σ, !wtabsizeG Σ, !wmemG Σ, !wmemsizeG Σ, !wglobG Σ, !wframeG Σ, !hvisG Σ, !hmsG Σ,
+        !logrel_na_invs Σ, HWP:host_program_logic}.
 
   Definition xx i := (VAL_int32 (Wasm_int.int_of_Z i32m i)).
   Definition xb b := (VAL_int32 (wasm_bool b)).
@@ -82,6 +84,10 @@ Section Examples.
     iApply wp_wasm_empty_ctx.
     iApply "Hes2". done.
   Qed.
+
+  Lemma wp_wand s E (e : iris.expr) (Φ Ψ : iris.val -> iProp Σ) :
+    WP e @ s; E {{ Φ }} -∗ (∀ v, Φ v -∗ Ψ v) -∗ WP e @ s; E {{ Ψ }}.
+  Proof. iApply (wp_wand). Qed.
   
   Definition lse a : iris.expr :=
     to_e_list
@@ -138,6 +144,14 @@ Section Examples.
       rewrite -(app_nil_l [_]).
       iApply (wp_invoke_native with "Hf Haf");eauto.
       iModIntro. iNext. iIntros "[Hf Haf]".
+      rewrite -wp_frame_rewrite.
+      iApply wp_wasm_empty_ctx_frame.
+      take_drop_app_rewrite 0.
+      iApply (wp_block_local_ctx with "Hf");[eauto..|].
+      iNext. iIntros "Hf".
+      iApply wp_wasm_empty_ctx_frame.
+      rewrite wp_frame_rewrite.
+      
       iApply fupd_wp.
       iMod ("Hcls" with "[$]") as "Hown". iModIntro.
       simpl.
@@ -163,8 +177,413 @@ Section Examples.
     iRight. iFrame. auto.
   Qed.
     
+
+  Definition not_host (cl : function_closure) : Prop :=
+    match cl with
+    | FC_func_host _ _ => False
+    | _ => True
+    end.
+  Definition no_host_cls (vs : seq.seq module_export) (wfs : gmap nat function_closure) :=
+    Forall (λ v, match modexp_desc v with
+            | MED_func (Mk_funcidx i0) => (∀ cl, wfs !! i0 = Some cl -> not_host cl)
+            | _ => True
+            end) vs.
+
+
+  Definition interp_closure_pre τctx i (τf : function_type) :=
+    λne (cl : leibnizO function_closure),
+         match cl with
+         | FC_func_native j τ' t_locs b_es =>
+             if instance_eqb i j then ⌜τf = τ' ∧
+                                        let 'Tf tn tm := τf in
+                                        be_typing (upd_local_label_return τctx (tn ++ t_locs) [tm] (Some tm)) b_es (Tf [] tm)⌝%I
+             else interp_closure (HWP:=HWP) τf cl
+         | _ => interp_closure (HWP:=HWP) τf cl
+         end.
+  Global Instance interp_closure_pre_persistent τctx i τf cl : Persistent (interp_closure_pre τctx i τf cl).
+  Proof. destruct cl,f;try apply _. simpl. destruct (instance_eqb i i0);apply _. Qed.
+  Global Instance interp_closure_persistent τf cl : Persistent (interp_closure (HWP:=HWP) τf cl).
+  Proof. destruct cl,f;try apply _. Qed.
+  
+  Definition interp_instance_pre (v_imps := seq.seq module_export) (τctx : t_context) :=
+    λne (i : leibnizO instance), interp_instance' τctx (interp_closure_pre τctx i) i.
+  Global Instance interp_instance_pre_persistent τctx i : Persistent (interp_instance_pre τctx i).
+  Proof. apply interp_instance_persistent';intros. destruct cl,f; apply _. Qed.
+
+  Lemma n_zeros_length l :
+    length (n_zeros l) = length l.
+  Proof.
+    induction l;auto. simpl. rewrite IHl. 
+    auto.
+  Qed.
+
+  Lemma n_zeros_interp_values l :
+    ⊢ ([∗ list] y1;y2 ∈ n_zeros l;l, interp_value (Σ:=Σ) y2 y1)%I.
+  Proof.
+    iApply big_sepL2_forall.
+    iSplit;[iPureIntro;apply n_zeros_length|].
+    iIntros (k z v Hz Hv).
+    unfold n_zeros in Hz.
+    apply lookup_lt_Some in Hv as Hlt.
+    apply take_drop_middle in Hv.
+    rewrite -Hv in Hz.
+    rewrite seq.map_cat seq.map_cons /= in Hz.
+    rewrite list_lookup_middle in Hz;simplify_eq.
+    { unfold interp_value. destruct v; iExists _;eauto. }
+    rewrite length_is_size size_map -length_is_size.
+    rewrite take_length. lia.
+  Qed.
+
+  Lemma interp_closure_pre_ind C i ft cl :
+    tc_label C = [] ∧ tc_return C = None ->
+    (□ ▷ interp_instance (HWP:=HWP) C i) -∗
+    interp_closure_pre C i ft cl -∗
+    interp_closure (HWP:=HWP) ft cl.
+  Proof.
+    iIntros (Hnil) "#IH #Hcl".
+    destruct cl.
+    { iSimpl in "Hcl".
+      destruct (instance_eqb i i0) eqn:Heq.
+      { iDestruct "Hcl" as "[-> Htyp]".
+        iSimpl. destruct f. iSplit;[auto|].
+        iDestruct "Htyp" as "%Htyp".
+        iModIntro.
+        iNext. revert Heq. move/eqP=>Heq. rewrite Heq.
+        iIntros (vcs) "Hv Hown". iIntros (f1) "Hf".
+        iDestruct "Hv" as "[%Hcontr|Hv]";[done|iDestruct "Hv" as (v' Heqv) "#Hv"].
+        iDestruct (be_fundamental_local with "IH") as "HH";eauto. inversion Heqv.
+        
+        iDestruct ("HH" $! _ (v' ++ n_zeros l) with "[$] [$] []") as "Hcont".
+        { iRight. iExists _. iSplit;[eauto|]. iApply big_sepL2_app;iFrame "#".
+          iApply n_zeros_interp_values. }
+        iSimpl in "Hcont".
+        iIntros (LI Hfill%lfilled_Ind_Equivalent).
+        inversion Hfill;inversion H9;simplify_eq.
+        repeat erewrite app_nil_l, app_nil_r.
+        iFrame. }
+      { destruct f. iDestruct "Hcl" as "[-> Hcl]".
+        iSplit;eauto. }
+    }
+    { simpl. auto. }
+  Qed.
+    
+  
+  Lemma interp_instance_pre_create τctx i :
+    (tc_label τctx) = [] ∧ (tc_return τctx) = None ->
+    interp_instance_pre τctx i -∗
+    interp_instance (HWP:=HWP) τctx i.
+  Proof.
+    iIntros (Hnil) "#Hpre".
+    iLöb as "IH".
+    set (IH := (▷ interp_instance τctx i)%I).
+    destruct τctx, i.
+    iDestruct "Hpre" as "[Htypes [Hfunc [Htable [Hmem Hglob]]]]".
+    iFrame "#".
+    iDestruct (big_sepL2_length with "Hfunc") as %Hlen.
+    iSplitR.
+    { iApply (big_sepL2_forall).
+      iSplit;[auto|iIntros (k f ft Hf Hft)].
+      iDestruct (big_sepL2_lookup with "Hfunc") as (cl) "[Hfna Hcl]";[eauto..|].
+      iExists _. iFrame "Hfna".
+      iApply interp_closure_pre_ind;eauto. }
+    { destruct (nth_error tc_table 0).
+      destruct (nth_error inst_tab 0);[|done].
+      iDestruct "Htable" as (table_size) "[Hsize Ht]".
+      iExists _. iFrame "Hsize".
+      iApply (big_sepL_forall).
+      iIntros (k x Hlook).
+      iDestruct (big_sepL_lookup with "Ht") as (τf fe) "[Htt Hf]";[eauto|].
+      iExists τf,_. iFrame "Htt".
+      destruct fe;[|auto].
+      iDestruct "Hf" as (?) "[Hfna Hf]".
+      iExists _. iFrame "Hfna". iApply interp_closure_pre_ind;eauto. done. }
+  Qed.
+      
+  Definition import_resources_wasm_typecheck_invs (v_imps: list module_export)
+             (t_imps: list extern_t) (wfs: gmap nat function_closure)
+             (wts: gmap nat tableinst) (wms: gmap nat memory) (wgs: gmap nat global): iProp Σ :=
+  [∗ list] i ↦ v; t ∈ v_imps; t_imps,
+  match v.(modexp_desc) with
+  | MED_func (Mk_funcidx i) => ((∃ cl, na_inv logrel_nais (wfN (N.of_nat i)) (N.of_nat i ↦[wf] cl) ∗ ⌜ wfs !! i = Some cl /\ t = ET_func (cl_type cl) ⌝)%I)
+                                
+  | MED_table (Mk_tableidx i) => (∃ tab, N.of_nat i ↪[wtsize]tab_size tab ∗
+                                                 ([∗ list] j↦tabelem ∈ table_data tab, na_inv logrel_nais (wtN (N.of_nat i) (N.of_nat j)) (N.of_nat i ↦[wt][N.of_nat j]tabelem))
+                                                 ∗ ⌜ wts !! i = Some tab /\ True ⌝)
+                                  
+  | MED_mem (Mk_memidx i) => (∃ mem, na_inv logrel_nais (wmN (N.of_nat i)) (N.of_nat i ↦[wmblock] mem) ∗ ⌜ wms !! i = Some mem /\ True⌝)
+                              
+  | MED_global (Mk_globalidx i) => (∃ g gt, na_inv logrel_nais (wgN (N.of_nat i)) (∃ w, N.of_nat i ↦[wg] Build_global (tg_mut gt) w ∗ interp_value (tg_t gt) w)
+                                                  ∗ ⌜ wgs !! i = Some g /\ t = ET_glob gt /\ global_agree g gt ⌝)
+  end.
+
+  Global Instance imports_invs_persistent v_imps t_imps wfs wts wms wgs : Persistent (import_resources_wasm_typecheck_invs v_imps t_imps wfs wts wms wgs).
+  Proof.
+    apply big_sepL2_persistent=>n exp expt.
+    destruct (modexp_desc exp);[destruct f;apply _|
+                                 destruct t;apply _|
+                                 destruct m;apply _|
+                                 destruct g;apply _].
+  Qed.
+
+
+  Lemma import_resources_wasm_typecheck_alloc E v_imps t_imps wfs wts wms wgs :
+    import_resources_wasm_typecheck v_imps t_imps wfs wts wms wgs ={E}=∗
+    import_resources_wasm_typecheck_invs v_imps t_imps wfs wts wms wgs.
+  Proof.
+    iIntros "Himps".
+    iApply big_sepL2_fupd.
+    iApply (big_sepL2_mono with "Himps");intros k exp expt Hlook1 Hlook2;simpl.
+    destruct (modexp_desc exp);[destruct f|destruct t|destruct m|destruct g];iIntros "Hres".
+    { iDestruct "Hres" as (cl) "[Hres ?]". iExists _. iFrame.
+      iApply na_inv_alloc. iNext. iFrame. }
+    { iDestruct "Hres" as (tab) "[[Hres ?] ?]". iExists _. iFrame.
+      iApply big_sepL_fupd.
+      iApply (big_sepL_mono with "Hres");intros k' el Hlook;simpl.
+      iIntros "Hn".
+      iApply na_inv_alloc. iNext;iFrame. }
+    { iDestruct "Hres" as (mem) "[Hres ?]". iExists _. iFrame.
+      iApply na_inv_alloc. iNext. iFrame. }
+    { iDestruct "Hres" as (g gt) "[Hres %]". iExists _,_. iFrame "%".
+      destruct H as (?&?&?).
+      iApply na_inv_alloc. iNext. iFrame.
+      destruct gt;simplify_eq. rewrite /global_agree /= in H1.
+      revert H1. move/andP =>[Hmut Htyp].
+      revert Htyp. move/eqP=>Htyp.
+      revert Hmut. move/eqP=>Hmut.
+      rewrite Htyp. destruct g;simplify_eq. simpl. iExists g_val. iFrame.
+      iApply interp_value_type_of. }
+  Qed.
+
+  Lemma import_resources_wasm_typecheck_func_len v_imps t_imps wfs wts wms wgs :
+    import_resources_wasm_typecheck v_imps t_imps wfs wts wms wgs -∗
+    ⌜length (ext_func_addrs (map (λ mexp : module_export, modexp_desc mexp) v_imps)) = length (ext_t_funcs t_imps)⌝.
+  Proof.
+    iIntros "Hi".
+    iDestruct (big_sepL2_length with "Hi") as %Hlen.
+    iInduction (v_imps) as [] "IH"
+  forall (t_imps Hlen).
+    { simpl. destruct t_imps;done. }
+    { destruct t_imps;[done|].
+      simpl in Hlen. inversion Hlen.
+      iDestruct "Hi" as "[Hx Hi]".
+      iDestruct ("IH" with "[] Hi") as %HlenIH;auto;iClear "Hi".
+      rewrite map_cons.
+      destruct (modexp_desc a).
+      { destruct f. simpl. rewrite HlenIH.
+        iDestruct "Hx" as (?) "[_ [_ %H]]".
+        rewrite H //. }
+      { destruct t. rewrite HlenIH. simpl. simpl. }
+      
+      simpl. 
+    }
     
     
+  
+  Definition module_inst_resources_func_invs (mfuncs: list module_func) (inst: instance) (inst_f: list funcaddr) : iProp Σ :=
+    ([∗ list] f; addr ∈ mfuncs; inst_f,
+       (* Allocated wasm resources *)
+       na_inv logrel_nais (wfN (N.of_nat addr))
+       (N.of_nat addr ↦[wf] (FC_func_native
+                              inst
+                              (nth match f.(modfunc_type) with
+                                   | Mk_typeidx k => k
+                                   end (inst.(inst_types)) (Tf [] []))
+                              f.(modfunc_locals)
+                                  f.(modfunc_body)))
+    )%I.
+
+  Lemma module_inst_resources_func_invs_alloc E mfuncs inst inst_f :
+    module_inst_resources_func mfuncs inst inst_f ={E}=∗
+    module_inst_resources_func_invs mfuncs inst inst_f .
+  Proof.
+    iIntros "Himps".
+    iApply big_sepL2_fupd.
+    iApply (big_sepL2_mono with "Himps");intros k exp expt Hlook1 Hlook2;simpl.
+    iIntros "Hf".
+    iApply na_inv_alloc. iNext. iFrame.
+  Qed.
+
+  Definition module_inst_resources_tab_invs (mtabs: list module_table) (inst_t: list tableaddr) : iProp Σ :=
+    ([∗ list] tab; addr ∈ mtabs; inst_t,
+       let tab := (match tab.(modtab_type).(tt_limits) with
+                                 | {| lim_min := min; lim_max := omax |} =>
+                                     (Build_tableinst
+                                        (repeat None (ssrnat.nat_of_bin min)))
+                                       (omax)
+                   end) in
+       N.of_nat addr ↪[wtsize]tab_size tab ∗
+       ([∗ list] j↦tabelem ∈ table_data tab, na_inv logrel_nais (wtN (N.of_nat addr) (N.of_nat j)) (N.of_nat addr ↦[wt][N.of_nat j]tabelem))       
+    )%I.
+
+  Lemma module_inst_resources_tab_invs_alloc E mtabs inst_t :
+    module_inst_resources_tab mtabs inst_t ={E}=∗
+    module_inst_resources_tab_invs mtabs inst_t.
+  Proof.
+    iIntros "Himps".
+    iApply big_sepL2_fupd.
+    iApply (big_sepL2_mono with "Himps");intros k exp expt Hlook1 Hlook2;simpl.
+    iIntros "[Hsize Hf]". iFrame.
+    iApply big_sepL_fupd.
+    iApply (big_sepL_mono with "Hsize");intros k' x Hx;simpl. iIntros "H".
+    iApply na_inv_alloc. iNext. iFrame.
+  Qed.
+
+  Definition module_inst_resources_mem_invs (mmems: list memory_type) (inst_m: list memaddr) : iProp Σ := 
+    ([∗ list] mem; addr ∈ mmems; inst_m,
+       na_inv logrel_nais (wmN (N.of_nat addr))
+       (N.of_nat addr ↦[wmblock] (match mem with
+                                 | {| lim_min:= min; lim_max := omax |} =>
+                                     Build_memory
+                                       {| ml_init := #00%byte; ml_data := repeat #00%byte (N.to_nat min) |}
+                                       (omax)
+                                 end))
+    ).
+
+  Lemma module_inst_resources_mem_invs_alloc E mmems inst_m :
+    module_inst_resources_mem mmems inst_m  ={E}=∗
+    module_inst_resources_mem_invs mmems inst_m.
+  Proof.
+    iIntros "Himps".
+    iApply big_sepL2_fupd.
+    iApply (big_sepL2_mono with "Himps");intros k exp expt Hlook1 Hlook2;simpl.
+    iIntros "Hf".
+    iApply na_inv_alloc. iNext. iFrame.
+  Qed.
+  
+  Definition module_inst_resources_glob_invs (mglobs: list module_glob) (g_inits: list value) (inst_g: list globaladdr) : iProp Σ :=
+    ([∗ list] g; addr ∈ mglobs; inst_g,
+       na_inv logrel_nais (wgN (N.of_nat addr)) (∃ w, N.of_nat addr ↦[wg] Build_global (tg_mut (modglob_type g)) w
+                                                               ∗ interp_value (tg_t (modglob_type g)) w)
+    ).
+
+  Lemma module_inst_resources_glob_invs_alloc E mglobs g_inits inst_g :
+    module_inst_resources_glob mglobs g_inits inst_g ={E}=∗
+    module_inst_resources_glob_invs mglobs g_inits inst_g.
+  Proof.
+    iIntros "Himps".
+    iApply big_sepL2_fupd.
+    iApply (big_sepL2_mono with "Himps");intros k exp expt Hlook1 Hlook2;simpl.
+    iIntros "Hf".
+    iApply na_inv_alloc. iNext. iExists _. iFrame.
+    (* TODO:fix once pulled *)
+  Admitted.  
+
+
+  
+  Lemma interp_instance_alloc_no_host E m t_imps t_exps v_imps wfs wts wms wgs g_inits inst :
+    module_typing m t_imps t_exps ->
+    (inst.(inst_types) = m.(mod_types) /\
+       let v_imp_descs := map (fun mexp => mexp.(modexp_desc)) v_imps in
+       prefix (ext_func_addrs v_imp_descs) inst.(inst_funcs) /\
+         prefix (ext_tab_addrs v_imp_descs) inst.(inst_tab) /\
+         prefix (ext_mem_addrs v_imp_descs) inst.(inst_memory) /\
+         prefix (ext_glob_addrs v_imp_descs) inst.(inst_globs)) ->
     
+    ([∗ map] _↦cl ∈ wfs, interp_closure (HWP:=HWP) (cl_type cl) cl)%I -∗ (* we must assume that the imported closures are valid *)
+    import_resources_wasm_typecheck v_imps t_imps wfs wts wms wgs -∗
+    module_inst_resources_wasm m inst g_inits
+    ={E}=∗ ∃ C, ⌜tc_label C = [] ∧ tc_local C = [] ∧ tc_return C = None⌝ ∗ interp_instance (HWP:=HWP) C inst.
+  Proof.
+    iIntros (Hmod Himps_of_inst) "#Himps_val Hir Hmr".
+    destruct Hmod as [fts [gts Hmod]].
+    set (ifts := ext_t_funcs t_imps).
+    set (its := ext_t_tabs t_imps).
+    set (ims := ext_t_mems t_imps).
+    set (igs := ext_t_globs t_imps).
+    set (C :=
+           {|
+             tc_types_t := (mod_types m);
+             tc_func_t := (ifts ++ fts)%list;
+             tc_global := (igs ++ gts)%list;
+             tc_table := (its ++ map (λ t : module_table, modtab_type t) (mod_tables m))%list;
+             tc_memory := (ims ++ (mod_mems m))%list;
+             tc_local := [];
+             tc_label := [];
+             tc_return := None
+           |}).
+
+    iExists C. iSplitR;[iModIntro;auto|].
+    iMod (import_resources_wasm_typecheck_alloc with "Hir") as "#Hir".
+    iDestruct "Hmr" as "(Hfr & Htr & Hmr & Hgr)".
+    iMod (module_inst_resources_func_invs_alloc with "Hfr") as "#Hfr".
+    iMod (module_inst_resources_tab_invs_alloc with "Htr") as "#Htr".
+    iMod (module_inst_resources_mem_invs_alloc with "Hmr") as "#Hmr".
+    iMod (module_inst_resources_glob_invs_alloc with "Hgr") as "#Hgr".
+    iModIntro.
     
+    iApply interp_instance_pre_create;[auto|].
+    unfold interp_instance_pre. destruct inst. rewrite /C.
+    (* destruct m. simpl in Hmod. *)
+    (* destruct Hmod as (Htypes & Htables & Hmems & Hglobals *)
+    (*                   & Helem & Hdata & Hstart & Himps & Hexps). *)
+    (* simpl in Himps_of_inst. simpl. *)
+    destruct Himps_of_inst as (Htypeq & Hprefunc & Hpretables & Hpremem & Hpreglob).
+    iSplitR.
+    { destruct m. simpl in Hmod.
+      simpl in *. auto. }
+    
+    iSplitR.
+    { iClear "Htr Hmr Hgr".
+      rewrite /ifts. iSimpl in "Hfr".
+      iDestruct (big_sepL2_length with "Hfr") as %Hlenfr.
+      iApply big_sepL2_forall. simpl in Hprefunc.
+      iDestruct (big_sepL2_length with "Hir") as %Himp_len.
+      destruct m. simpl in Hmod.
+      destruct Hmod as (Htypes & Htables & Hmems & Hglobals
+                        & Helem & Hdata & Hstart & Himps & Hexps).
+      simpl in *.
+      apply Forall2_length in Htypes as Hlenfr'. rewrite Hlenfr' in Hlenfr.
+      
+      
+      simplify_eq. simpl.
+
+      
+      rewrite -(take_drop (get_import_func_count m) inst_funcs).
+      iApply big_sepL2_app.
+      
+      unfold ext_t_funcs.
+
+
+      unfold get_import_func_count.
+      
+      rewrite -/(ext_t_funcs _).
+
+      
+      iApply big_sepL2_forall.
+
+    }
+    
+    simpl.
+    iSplitR.
+    { iPureIntro. }
+
+    
+                                    
+  (* Lemma instantiation_spec_operational (s: stuckness) E (hs_mod: N) (hs_imps: list vimp) (v_imps: list module_export) (hs_exps: list vi) (m: module) t_imps t_exps: *)
+(*   module_typing m t_imps t_exps -> *)
+(*   ∀ wfs wts wms wgs, *)
+(*   hs_mod ↪[mods] m -∗ *)
+(*   import_resources_host hs_imps v_imps -∗ *)
+(*   import_resources_wasm_typecheck v_imps t_imps wfs wts wms wgs -∗ *)
+(*   export_ownership_host hs_exps -∗ *)
+(*   WP (([:: ID_instantiate hs_exps hs_mod hs_imps], [::]): host_expr) @ s; E *)
+(*   {{ v, hs_mod ↪[mods] m ∗ *)
+(*         import_resources_host hs_imps v_imps ∗ (* vis, for the imports stored in host *) *)
+(*         import_resources_wasm_typecheck v_imps t_imps wfs wts wms wgs ∗ (* locations in the wasm store and type-checks *) *)
+(*         ∃ inst g_inits, *)
+(*           ⌜ inst.(inst_types) = m.(mod_types) /\ *)
+(*           (* We know what the imported part of the instance must be. *) *)
+(*           let v_imp_descs := map (fun mexp => mexp.(modexp_desc)) v_imps in *)
+(*           prefix (ext_func_addrs v_imp_descs) inst.(inst_funcs) /\ *)
+(*           prefix (ext_tab_addrs v_imp_descs) inst.(inst_tab) /\ *)
+(*           prefix (ext_mem_addrs v_imp_descs) inst.(inst_memory) /\ *)
+(*           prefix (ext_glob_addrs v_imp_descs) inst.(inst_globs) *)
+(*           ⌝ ∗ *)
+(*           module_inst_resources_wasm m inst g_inits ∗ (* allocated wasm resources. This also specifies the information about the newly allocated part of the instance. *) *)
+(*           module_export_resources_host v_imps hs_exps m.(mod_exports) inst (* export resources, in the host store *) *)
+(*           (* missing the constraints for the initialised globals. A wp (in wasm) for each of them in the future. Omitted *)
+(*              for now since we can just forbid the initialization of globals anyway *)                                                                                       *)
+(*   }}. *)
+(* Proof. *)
+
 End Examples.
